LambdaGraph/Algorithms.lean
@@ -1,0 +1,369 @@
+module
+
+import Std.Data.HashSet
+public import Std.Data.HashSet.Basic
+
+import LambdaGraph.Finset
+public import LambdaGraph.Nest
+
+def Expr.locals : Expr → Std.HashSet Nat × Std.HashSet Nat
+  | var n => ({n}, ∅)
+  | fn n => (∅, {n})
+  | const _ => (∅, ∅)
+  | bin _ e₁ e₂ =>
+    let (v₁, f₁) := e₁.locals
+    let (v₂, f₂) := e₂.locals
+    (v₁ ∪ v₂, f₁ ∪ f₂)
+  | cond c et ef =>
+    let (vc, fc) := c.locals
+    let (vt, ft) := et.locals
+    let (vf, ff) := ef.locals
+    (vc ∪ vt ∪ vf, fc ∪ ft ∪ ff)
+  | proj e _ => e.locals
+
+theorem Expr.var_in_locals_iff {e : Expr} {n : Nat} :
+    n ∈ e.locals.1 ↔ e.LocalVar n := by
+  constructor <;> intro h <;> fun_induction locals <;>
+    grind [Std.HashSet.singleton_eq_insert, Std.HashSet.mem_union_iff]
+
+theorem Expr.fn_in_locals_iff {e : Expr} {n : Nat} :
+    n ∈ e.locals.2 ↔ e.LocalFn n := by
+  constructor <;> intro h <;> fun_induction locals <;>
+    grind [Std.HashSet.singleton_eq_insert, Std.HashSet.mem_union_iff]
+
+instance {e : Expr} {n : Nat} {r : RefKind} : Decidable (e.Local n r) :=
+  match r with
+  | .var => decidable_of_bool (e.locals.1.contains n) Expr.var_in_locals_iff
+  | .fn => decidable_of_bool (e.locals.2.contains n) Expr.fn_in_locals_iff
+
+instance {e : Expr} {q : Nat → RefKind → Prop} [DecidableRel q] :
+    Decidable (∀ n r, e.Local n r → q n r) :=
+  let (eq := hlc) (lv, lf) := e.locals
+  decidable_of_bool (lv.all (decide <| q · .var) && lf.all (decide <| q · .fn)) <| by
+    grind [cases RefKind, Expr.var_in_locals_iff, Expr.fn_in_locals_iff,
+      Std.HashSet.all_eq_true_iff_forall_mem]
+
+instance {e : Expr} {n : Nat} : Decidable (e.Bounded n) :=
+  inferInstanceAs (Decidable (∀ m r, e.Local m r → m < n))
+
+inductive Path (p : Program) : Nat → Nat → Type where
+  | refl n : n < p.size → Path p n n
+  | step m n k : m ⟶[p] n → Path p n k → Path p m k
+
+def Path.length {p : Program} {m n : Nat} : Path p m n → Nat
+  | refl _ _ => 0
+  | step _ _ _ _ path => path.length + 1
+
+def Path.labels {p : Program} {m n : Nat} : Path p m n → Finset
+  | refl n _ => {n}
+  | step n _ _ _ path => path.labels.insert n
+
+inductive Path.Mem {p : Program} (l : Nat) : ∀ {m n}, Path p m n → Prop where
+  | head n (path : Path p l n) : path.Mem l
+  | tail m n k hs (path : Path p n k) : path.Mem l → (path.step m n k hs).Mem l
+
+instance {p : Program} {m n : Nat} : Membership Nat (Path p m n) where
+  mem path l := path.Mem l
+
+@[simp, grind =]
+theorem Path.length_refl {p : Program} {n : Nat} (hn : n < p.size) :
+    (Path.refl n hn).length = 0 := by simp [length]
+
+@[simp, grind =]
+theorem Path.length_step {p : Program} {m n k : Nat} {path : Path p n k}
+    (h : m ⟶[p] n) : (path.step _ _ _ h).length = path.length + 1 := by
+  simp [length]
+
+@[simp, grind =]
+theorem Path.mem_refl_iff {p : Program} {l n : Nat} (hn : n < p.size) :
+    l ∈ Path.refl n hn ↔ l = n := by
+  constructor
+  · intro h
+    have .head _ _ := h
+    rfl
+  · intro rfl
+    constructor
+
+@[simp, grind =]
+theorem Path.mem_step_iff {p : Program} {l m n k : Nat} {path : Path p n k}
+    (hs : m ⟶[p] n) : l ∈ path.step _ _ _ hs ↔ l = m ∨ l ∈ path := by
+  constructor
+  · intro h
+    cases h with
+    | head _ _ => exact .inl rfl
+    | tail _ _ _ _ _ h => exact .inr h
+  · rintro (rfl | h) <;> constructor <;> assumption
+
+theorem Path.lt_size_of_mem {p : Program} {l m n : Nat} {path : Path p m n}
+    (h : l ∈ path) : l < p.size := by
+  induction h with
+  | head n path =>
+    cases path with
+    | refl _ hl => exact hl
+    | step _ m _ hs path => exact hs.1
+  | tail m n k hs path h hl => exact hl
+
+theorem Path.lt_size_right {p : Program} {m n : Nat} (path : Path p m n) :
+    n < p.size := by
+  induction path with
+  | refl n hn => exact hn
+  | step m k n hs path ih => exact ih
+
+theorem Path.labels_correct {p : Program} {l m n : Nat} {path : Path p m n} :
+    l ∈ path.labels ↔ l ∈ path := by
+  constructor <;> intro h
+  · fun_induction labels
+    next n hn =>
+      simp only [Finset.singleton_eq_insert, Finset.mem_insert_iff,
+        Finset.notMem_emptyCollection, or_false] at h
+      subst n
+      constructor
+    next k m n hs path ih =>
+      simp only [Finset.mem_insert_iff] at h
+      obtain rfl | h := h
+      · constructor
+      · apply_rules [Mem.tail]
+  · induction h with grind [labels, cases Path]
+
+def Path.push {p : Program} {m n k : Nat} (path : Path p m n) (hk : k < p.size)
+    (h : n ⟶[p] k) : Path p m k :=
+  match path with
+  | refl _ hm => .step _ _ _ h (.refl _ hk)
+  | step _ _ _ hs path => .step _ _ _ hs (path.push hk h)
+
+@[simp, grind =]
+theorem Path.length_push {p : Program} {m n k : Nat} {path : Path p m n}
+    (hk : k < p.size) (h : n ⟶[p] k) :
+    (path.push hk h).length = path.length + 1 := by
+  induction path with simp [length, push, *]
+
+@[simp, grind =]
+theorem Path.mem_push_iff {p : Program} {l m n k : Nat} {path : Path p m n}
+    (hk : k < p.size) (h : n ⟶[p] k) :
+    l ∈ path.push hk h ↔ l ∈ path ∨ l = k := by
+  induction path with grind [push]
+
+theorem Path.split_last {p : Program} {m n : Nat} (path : Path p m n) :
+    (∃ (h : m = n) (hm : m < p.size), path = h ▸ .refl _ hm) ∨
+      ∃ k hk h, ∃ path' : Path p m k, path = path'.push hk h := by
+  induction path with
+  | refl m hm => exact .inl ⟨rfl, hm, rfl⟩
+  | step m k n hs path ih =>
+    obtain ⟨rfl, hm, rfl⟩ | ⟨l, hn, hs', path, rfl⟩ := ih
+    · exact .inr ⟨_, hm, hs, .refl _ hs.1, rfl⟩
+    · exact .inr ⟨_, hn, hs', .step _ _ _ hs path, rfl⟩
+
+inductive Path.Acyclic {p : Program} : ∀ {m n}, Path p m n → Prop where
+  | refl n hn : (Path.refl n hn).Acyclic
+  | step m n k hs (path : Path p n k) :
+    m ∉ path → path.Acyclic → (path.step m n k hs).Acyclic
+
+theorem Path.size_labels_eq_of_acyclic {p : Program} {m n : Nat}
+    {path : Path p m n} (h : path.Acyclic) :
+    path.labels.size = path.length + 1 := by
+  induction h with
+    simp_all! [labels_correct, Finset.size_insert_of_mem,
+      Finset.size_insert_of_notMem]
+
+theorem Path.length_lt_size_of_acyclic {p : Program} {m n : Nat}
+    {path : Path p m n} (h : path.Acyclic) : path.length < p.size := by
+  apply Nat.lt_of_succ_le
+  simp only [Nat.succ_eq_add_one, ← size_labels_eq_of_acyclic h]
+  apply Finset.size_le_of_all_lt
+  intro k
+  rw [labels_correct]
+  exact lt_size_of_mem
+
+theorem Path.exists_of_mem {p : Program} {l m n : Nat} {path : Path p m n}
+    (h : l ∈ path) : ∃ (path' : Path p l n),
+      path'.length ≤ path.length ∧ ∀ k ∈ path', k ∈ path := by
+  induction h with grind
+
+theorem Path.exists_acyclic.aux {p : Program} {b m n : Nat} {path : Path p m n}
+    (hb : path.length ≤ b) : ∃ (path' : Path p m n),
+      path'.Acyclic ∧ ∀ l ∈ path', l ∈ path := by
+  induction b generalizing m n path with
+  | zero =>
+    cases path with
+    | refl _ hm => exact ⟨.refl m hm, .refl m hm, fun _ h => h⟩
+    | step _ k n hs path => simp [length] at hb
+  | succ b ih =>
+    cases path with
+    | refl _ hm => exact ⟨.refl m hm, .refl m hm, fun _ h => h⟩
+    | step _ k n hs path =>
+      simp only [length, Nat.add_le_add_iff_right] at hb
+      by_cases hm : m ∈ path
+      · obtain ⟨path', hlen, h⟩ := exists_of_mem hm
+        grind
+      · obtain ⟨path', ha, h⟩ := ih hb
+        replace hm : m ∉ path' := fun hm' => hm (h _ hm')
+        refine ⟨.step m k n hs path', .step _ _ _ _ _ hm ha, ?_⟩
+        grind
+
+theorem Path.exists_acyclic {p : Program} {m n : Nat} (path : Path p m n) :
+    ∃ (path' : Path p m n), path'.Acyclic ∧ ∀ l ∈ path', l ∈ path :=
+  exists_acyclic.aux (Nat.le_refl _)
+
+theorem Program.pathWithout_iff {p : Program} {m n k : Nat} (hk : k < p.size) :
+    m ⟶[p, n]* k ↔ ∃ path : Path p m k, n ∉ path := by
+  constructor
+  · intro h
+    induction h with
+    | refl m hne =>
+      exists .refl _ hk
+      grind
+    | step m l k hne hs h ih =>
+      obtain ⟨path, hn⟩ := ih hk
+      exists .step _ _ _ hs path
+      grind
+  · rintro ⟨path, h⟩
+    induction path with grind [intro PathWithout]
+
+theorem Expr.free_iff' {p : Program} {e : Expr} {n : Nat} :
+    e.Free p n ↔
+      e.LocalVar n ∨ ∃ (m k : Nat) (path : Path p m k),
+        e.LocalFn m ∧ (p.fn[k]'path.lt_size_right).LocalVar n ∧ n ∉ path ∧
+        path.length < p.size := by
+  constructor
+  · intro hf
+    obtain hlv | ⟨m, k, hk, hlf, hpath, hlv⟩ := free_iff.mp hf
+    · exact .inl hlv
+    · obtain ⟨path, hn⟩ := (Program.pathWithout_iff hk).mp hpath
+      obtain ⟨path', ha, h⟩ := path.exists_acyclic
+      have hlen := Path.length_lt_size_of_acyclic ha
+      exact .inr ⟨m, k, path', hlf, hlv, fun hn' => hn (h _ hn'), hlen⟩
+  · rintro (hlv | ⟨m, k, path, hlf, hlv, hn, hlen⟩)
+    · exact free_of_localVar hlv
+    · have hk := path.lt_size_right
+      have hpath := (Program.pathWithout_iff hk).mpr ⟨path, hn⟩
+      exact free_iff.mpr <| .inr ⟨m, k, hk, hlf, hpath, hlv⟩
+
+def flatMap (s : Std.HashSet Nat) (f : Nat → Std.HashSet Nat) : Std.HashSet Nat :=
+  aux ∅ s.toList
+  where
+    aux s
+      | [] => s
+      | n :: ns => aux (s ∪ f n) ns
+
+@[simp, grind =]
+theorem mem_flatMap_iff {s : Std.HashSet Nat} {f : Nat → Std.HashSet Nat}
+    {n : Nat} : n ∈ flatMap s f ↔ ∃ m ∈ s, n ∈ f m := by
+  suffices ∀ t l, n ∈ flatMap.aux f t l ↔ n ∈ t ∨ ∃ m ∈ l, n ∈ f m by
+    replace := this ∅ s.toList
+    simpa
+  intro t l
+  induction l generalizing t with grind [flatMap.aux, Std.HashSet.mem_union_iff]
+
+@[simp, grind =]
+theorem mem_union_iff {s₁ s₂ : Std.HashSet Nat} {n : Nat} :
+    n ∈ s₁ ∪ s₂ ↔ n ∈ s₁ ∨ n ∈ s₂ := by grind [Std.HashSet.mem_union_iff]
+
+public section
+
+def Program.fnFreeVars (p : Program) : Vector (Std.HashSet Nat) p.size :=
+  let (lvs, lfs) := Vector.ofFn (p.fn[·].locals) |>.unzip
+  aux lfs lvs p.size
+  where
+    aux lfs v : Nat → _
+      | 0 => v
+      | n + 1 =>
+        let update free lf :=
+          free ∪ flatMap lf fun m =>
+            if hm : m < p.size then v[m].erase m else ∅
+        aux lfs (v.zipWith update lfs) n
+
+theorem Program.fnFreeVars_correct {p : Program} {m n : Nat} (hm : m < p.size) :
+    n ∈ p.fnFreeVars[m] ↔ p.fn[m].Free p n := by
+  let (eq := hlc) (lvs, lfs) := Vector.ofFn (n := p.size) (p.fn[·].locals) |>.unzip
+  have hlvs : ∀ {i} (hi : i < p.size) k, k ∈ lvs[i] ↔ p.fn[i].LocalVar k := by
+    grind [Expr.var_in_locals_iff]
+  have hlfs : ∀ {i} (hi : i < p.size) k, k ∈ lfs[i] ↔ p.fn[i].LocalFn k := by
+    grind [Expr.fn_in_locals_iff]
+  suffices ∀ v i, n ∈ (fnFreeVars.aux p lfs v i)[m]'hm ↔
+      n ∈ v[m] ∨ ∃ (k l : Nat) (path : Path p k l), p.fn[m].LocalFn k ∧
+        n ∈ v[l]'path.lt_size_right ∧ n ∉ path ∧ path.length < i by
+    have := this lvs p.size
+    unfold fnFreeVars
+    rw [hlc, this]
+    simp only [hlvs, Expr.free_iff']
+  intro v i
+  induction i generalizing v with
+  | zero => grind [fnFreeVars.aux]
+  | succ i ih =>
+    let update free lf :=
+      free ∪ flatMap lf fun m =>
+        if hm : m < p.size then v[m].erase m else ∅
+    specialize ih (v.zipWith update lfs)
+    constructor
+    · intro h
+      obtain hn | ⟨k, l, path, hlf, hn, hmem, hlen⟩ := ih.mp h <;>
+        simp only [Vector.getElem_zipWith, mem_union_iff, mem_flatMap_iff, update] at hn
+      · obtain hn | ⟨k, hlf, hn⟩ := hn
+        · exact .inl hn
+        · rw [hlfs] at hlf
+          have hk : k < p.size := by grind
+          simp only [hk, ↓reduceDIte, Std.HashSet.mem_erase, beq_eq_false_iff_ne, ne_eq] at hn
+          obtain ⟨hne, hn⟩ := hn
+          exact .inr <| ⟨_, _, .refl _ hk, hlf, hn, by grind⟩
+      · obtain hn | ⟨o, hlf', hn⟩ := hn
+        · exact .inr ⟨_, _, path, hlf, hn, hmem, by lia⟩
+        · rw [hlfs] at hlf'
+          have hl := path.lt_size_right
+          have ho : o < p.size := by grind
+          simp only [ho, ↓reduceDIte, Std.HashSet.mem_erase, beq_eq_false_iff_ne, ne_eq] at hn
+          obtain ⟨hne, hn⟩ := hn
+          exact .inr <| ⟨_, _, path.push ho ⟨hl, hlf'⟩, hlf, hn, by grind⟩
+    · rintro (hn | ⟨k, l, path, hlf, hn, hmem, hlen⟩)
+      · simp [fnFreeVars.aux, update, *]
+      · have hl := path.lt_size_right
+        obtain h | ⟨o, ho, hs, path, rfl⟩ := path.split_last
+        · grind [fnFreeVars.aux]
+        · simp only [Path.length_push, Nat.add_lt_add_iff_right] at hlen
+          have ho := path.lt_size_right
+          have hn' : n ∈ (v.zipWith update lfs)[o] := by grind [Succ]
+          exact ih.mpr <| .inr ⟨_, _, path, hlf, hn', by grind, hlen⟩
+
+def Expr.freeVars (e : Expr) (p : Program) :=
+  let (lv, lf) := e.locals
+  let ffs := p.fnFreeVars
+  lv ∪ flatMap lf fun m => if hm : m < p.size then ffs[m].erase m else ∅
+
+theorem Expr.freeVars_correct {p : Program} {e : Expr} {n : Nat} :
+    n ∈ e.freeVars p ↔ e.Free p n := by
+  simp only [freeVars, mem_union_iff, var_in_locals_iff, mem_flatMap_iff, fn_in_locals_iff]
+  constructor
+  · rintro (hlv | ⟨m, hlf, hn⟩)
+    · exact free_of_localVar hlv
+    · have hm : m < p.size := by grind
+      simp only [hm, ↓reduceDIte, Std.HashSet.mem_erase, beq_eq_false_iff_ne,
+        Program.fnFreeVars_correct] at hn
+      obtain ⟨hne, hf⟩ := hn
+      exact free_of_localFn_of_free hm hne.symm hlf hf
+  · intro hf
+    obtain hlv | ⟨m, k, hk, hlf, hpath, hlv⟩ := free_iff.mp hf
+    · exact .inl hlv
+    · have hm : m < p.size := by cases hpath <;> grind [Program.Succ]
+      refine .inr ⟨m, hlf, ?_⟩
+      simp only [hm, ↓reduceDIte, Std.HashSet.mem_erase, beq_eq_false_iff_ne,
+        Program.fnFreeVars_correct]
+      have hne := hpath.ne_start
+      exact ⟨hne.symm, (Program.free_in_fn_iff hm hne).mpr ⟨_, hk, hlv, hpath⟩⟩
+
+instance {p : Program} {e : Expr} {n : Nat} : Decidable (e.Free p n) :=
+  decidable_of_bool ((e.freeVars  p).contains n) Expr.freeVars_correct
+
+instance {p : Program} {e : Expr} {q : Nat → Prop} [DecidablePred q] :
+    Decidable (∀ n, e.Free p n → q n) :=
+  decidable_of_bool ((e.freeVars p).all (decide <| q ·)) <| by
+    simp [Expr.freeVars_correct, Std.HashSet.all_eq_true_iff_forall_mem]
+
+instance {p : Program} {e : Expr} : Decidable (e.Closed p) :=
+  inferInstanceAs (Decidable (∀ n, ¬e.Free p n))
+
+instance {c : Computation} {n : Nat} : Decidable (c.Free n) :=
+  inferInstanceAs (Decidable (c.expr.Free c.toProgram n))
+
+instance {c : Computation} : Decidable c.Closed :=
+  inferInstanceAs (Decidable (c.expr.Closed c.toProgram))
+
+end
